CoqOfRust/core/ops/links/range.v
@@ -2,10 +2,10 @@ Require Import CoqOfRust.CoqOfRust.
 Require Import links.M.
 
 (*
-pub struct Range<Idx> {
-    pub start: Idx,
-    pub end: Idx,
-}
+  pub struct Range<Idx> {
+      pub start: Idx,
+      pub end: Idx,
+  }
 *)
 Module Range.
   Record t {Idx : Set} : Set := {
@@ -24,3 +24,78 @@ Module Range.
       ];
   }.
 End Range.
+
+(*
+  pub enum Bound<T> {
+    Included(T),
+    Excluded(T),
+    Unbounded,
+  }
+*)
+Module Bound.
+  Inductive t {T : Set} : Set :=
+  | Included : T -> t
+  | Excluded : T -> t
+  | Unbounded : t.
+  Arguments t : clear implicits.
+
+  Global Instance IsLink {T : Set} `{Link T} : Link (t T) := {
+    Φ := Ty.apply (Ty.path "core::ops::Range::Bound") [] [Φ T];
+    φ x :=
+      match x with
+      | Included x => Value.StructTuple "core::ops::Range::Bound::Included" [φ x]
+      | Excluded x => Value.StructTuple "core::ops::Range::Bound::Excluded" [φ x]
+      | Unbounded => Value.StructTuple "core::ops::Range::Bound::Unbounded" []
+      end;
+  }.
+End Bound.
+
+(*
+  pub trait RangeBounds<T: ?Sized> {
+    fn start_bound(&self) -> Bound<&T>;
+    fn end_bound(&self) -> Bound<&T>;
+    fn contains<U>(&self, item: &U) -> bool
+    where
+        T: PartialOrd<U>,
+        U: ?Sized + PartialOrd<T>
+    fn is_empty(&self) -> bool
+    where
+        T: PartialOrd
+  }
+*)
+Module RangeBounds.
+  Definition run_start_bound 
+      (Self : Set) `{Link Self} 
+      (T : Set) `{Link T} : Set :=
+    { start_bound @ 
+      IsTraitMethod.t "core::ops::range::RangeBounds" [] [Φ T] (Φ Self) "start_bound" start_bound *
+      forall (self : Ref.t Pointer.Kind.Ref Self),
+        {{ start_bound [] [] [ φ self ] 🔽 (Bound.t (Ref.t Pointer.Kind.Ref T)) }}
+    }.
+
+  Definition run_end_bound 
+    (Self : Set) `{Link Self} 
+    (T : Set) `{Link T} : Set :=
+  { end_bound @ 
+    IsTraitMethod.t "core::ops::range::RangeBounds" [] [Φ T] (Φ Self) "end_bound" end_bound *
+    forall (self : Ref.t Pointer.Kind.Ref Self),
+      {{ end_bound [] [] [ φ self ] 🔽 (Bound.t (Ref.t Pointer.Kind.Ref T)) }}
+  }.
+
+  Definition run_contains
+    (Self : Set) `{Link Self} 
+    (T : Set) `{Link T} : Set :=
+  { contains @ 
+    IsTraitMethod.t "core::ops::range::RangeBounds" [] [Φ T] (Φ Self) "contains" contains *
+    forall (U : Set) `{Link U} (self : Ref.t Pointer.Kind.Ref Self) (item : Ref.t Pointer.Kind.Ref U),
+      {{ contains [] [Φ U] [ φ self; φ item ] 🔽 bool }}
+  }.
+
+  Record Run
+      (Self : Set) `{Link Self}
+      {T : Set} `{Link T} :
+    Set := {
+      start_bound : run_start_bound Self T;
+      end_bound : run_end_bound Self T;
+    }.
+End RangeBounds.
