CoqOfRust/revm/revm_bytecode/eof/links/header.v
@@ -1,7 +1,9 @@
 Require Import CoqOfRust.CoqOfRust.
 Require Import links.M.
-Require alloc.links.alloc.
-Require alloc.vec.links.mod.
+Require Import alloc.links.alloc.
+Require Import alloc.vec.links.mod.
+Require Import alloc.vec.links.mod.
+Require Import revm_bytecode.eof.header.
 
 Module EofHeader.
   Record t : Set := {
@@ -25,4 +27,20 @@ Module EofHeader.
         ("sum_container_sizes", φ sum_container_sizes)
       ]
   }.
+
+  Definition of_ty : OfTy.t (Ty.path "revm_bytecode::eof::header::EofHeader").
+  Proof. eapply OfTy.Make with (A := t); reflexivity. Defined.
+  Smpl Add apply of_ty : of_ty.
 End EofHeader.
+
+Module Impl_EofHeader.
+
+  Definition Self : Set := EofHeader.t.
+
+  (*
+    pub fn encode(&self, buffer: &mut Vec<u8>)
+  *)
+  Instance run_encode (self : Ref.t Pointer.Kind.Ref Self) (buffer : Ref.t Pointer.Kind.MutPointer (Vec.t U8.t Global.t)) :
+    Run.Trait header.eof.header.Impl_revm_bytecode_eof_header_EofHeader.encode [] [] [φ self; φ buffer] unit.
+  Admitted.
+End Impl_EofHeader.
